\documentclass{article}
\usepackage[utf8]{inputenc}
\usepackage[russian]{babel}

\begin{document}
\begin{center}
\section*{Доказательство формулы S K K = I}

$S\;K\;K = (\lambda x\;y\;z.x\;z\;(y\;z))\;(\lambda x\;y.x)\;(\lambda x\;y.x) \to_\beta \\
\lambda x\;y\;z.[x:=\lambda x\;y.x]\;z\;([y:=\lambda x\;y.x]\;z)=\lambda z. (\lambda x\;y.x)\;z\; ((\lambda x\;y.x)\;z)\to_\beta\\
\lambda z. ((\lambda y.z)\;(\lambda y.z)) \to_\beta \lambda z. (\lambda y.z[y:=\lambda y_1.z_1]) = \lambda z.z=I$

\end{center}
\end{document}
