\documentclass{article}
\usepackage[utf8]{inputenc}
\usepackage[russian]{babel}

\begin{document}
\begin{center}
\section*{Редукция лямбда-терма}
$((\lambda a.(\lambda b.b\; b)\; (\lambda b.b\; b))\; b)\; ((\lambda c.(c\; b))\; (\lambda a.a))) \to_\beta$ \\
$((\lambda a.(\lambda b.b\; b)\; (\lambda b.b\; b)[a := b])\; (\lambda c.(c[c := \lambda a.a]\; b)) = ((\lambda b.b\; b)(\lambda b.b\; b))(\lambda a.a\; b) \to_\beta$ \\
$((\lambda b.b\; b)(\lambda b.b\; b))(\lambda a.a [a := b]) = \Omega\; b$
\end{center}
\end{document}
